Add while loop laws

utp_rel.thy
@@ -79,6 +79,14 @@ definition ndet_assign :: "('a \<Longrightarrow> 's) \<Rightarrow> 's rel" where
 syntax "_ndet_assign" :: "svid \<Rightarrow> logic" ("_ := *" [75] 76)
 translations "_ndet_assign x" == "CONST ndet_assign x"
 
+definition while_top :: "'s pred \<Rightarrow> 's rel \<Rightarrow> 's rel" ("while\<^sup>\<top> _ do _ od") where 
+"while_top b P = (\<nu> X \<bullet> ((P ;; X) \<^bold>\<lhd> b \<^bold>\<rhd> II))"
+
+notation while_top ("while _ do _ od")
+
+definition while_bot :: "'s pred \<Rightarrow> 's rel \<Rightarrow> 's rel" ("while\<^sub>\<bottom> _ do _ od") where 
+"while_bot b P = (\<mu> X \<bullet> ((P ;; X) \<^bold>\<lhd> b \<^bold>\<rhd> II))"
+
 definition pre :: "('s\<^sub>1 \<leftrightarrow> 's\<^sub>2) \<Rightarrow> ('s\<^sub>1 \<Rightarrow> bool)" 
   where "pre P = \<lbrakk>Domain P\<rbrakk>\<^sub>P"
 
